first commit of branch for explicit existential types

FiatFormal/Language/Eval.v
@@ -1,353 +1,183 @@
 
-Require Export FiatFormal.Language.SubstExpExp.
-Require Export FiatFormal.Language.Step.
-Require Export FiatFormal.Language.Exp.
 Require Import FiatFormal.Language.Preservation.
+Require Export FiatFormal.Language.Step.
+Require Export FiatFormal.Language.SubstExpExp.
+Require Export FiatFormal.Language.SubstTypeExp.
 Require Import FiatFormal.Language.TyJudge.
+Require Export FiatFormal.Language.Exp.
 
 
+(********************************************************************)
 (* Big Step Evaluation
    This is also called 'Natural Semantics'.
    It provides a relation between the expression to be reduced
-   and its final value. *)
-Inductive EVAL : adt_defs -> exp -> exp -> Prop :=
- | EvDone
-   : forall adt_ds v2,
-     wnfX  v2
-     -> EVAL adt_ds v2 v2
+   and its final value.
+ *)
+Inductive EVAL : exp -> exp -> Prop :=
+ | EVDone
+   :  forall v2
+   ,  wnfX v2
+   -> EVAL v2 v2
 
- (* | EvLamApp *)
- (*   :  forall adt_ds x1 t11 x12 x2 v2 v3, *)
- (*     EVAL adt_ds x1 (XLam t11 x12) *)
- (*     -> EVAL adt_ds x2 v2 *)
- (*     -> EVAL adt_ds (substX 0 v2 x12) v3 *)
- (*     -> EVAL adt_ds (XApp x1 x2)      v3 *)
+ | EVLAMAPP
+   : forall x1 x12 t2 v3
+   ,  EVAL x1 (XLAM x12)     -> EVAL (substTX 0 t2 x12) v3
+   -> EVAL (XAPP x1 t2) v3
 
- | EvFixApp
-   : forall adt_ds t1 t2 x0 x1 x2 v2 v3,
-     EVAL adt_ds x0 (XFix t1 t2 x1)
-     -> EVAL adt_ds x2 v2
-     -> EVAL adt_ds (substX 0 (XFix t1 t2 x1) (substX 0 v2 x1)) v3
-     -> EVAL adt_ds (XApp x0 x2) v3
-
- | EvCon
-   : forall adt_ds dc xs vs,
-     EVALS adt_ds xs vs
-     -> EVAL adt_ds (XCon dc xs) (XCon dc vs)
-
- | EvMatch
-   :  forall adt_ds x1 x2 v3 dc vs alts tsArgs,
-     EVAL adt_ds x1 (XCon dc vs)
-     -> Forall wnfX vs
-     -> getAlt dc alts = Some (AAlt dc tsArgs x2)
-     -> EVAL adt_ds (substXs 0 vs x2) v3
-     -> EVAL adt_ds (XMatch x1 alts)   v3
-
- | EvChoice
-   : forall adt_ds x1 v2 t1 xs fp,
-     EVAL adt_ds x1 (XChoice t1 xs fp)
-     -> wnfX v2
-     (* -> fp v2 *) (* TODO *)
-     -> EVAL adt_ds x1 v2
-
- | EvCall
-   : forall adt_ds ac n xbody v1 xs vs,
-     EVALS adt_ds xs vs
-     -> Forall wnfX vs
-     -> getADTBody ac n adt_ds = Some xbody
-     -> EVAL adt_ds (substXs 0 vs xbody) v1
-     -> EVAL adt_ds (XCall ac n xs) v1
-
- with EVALS : adt_defs -> list exp -> list exp -> Prop :=
-      | EvsNil : forall adt_ds,
-          EVALS adt_ds nil nil
-
-      | EvsCons
-        :  forall adt_ds x v xs vs,
-          EVAL adt_ds  x  v
-           -> EVALS adt_ds xs vs
-           -> EVALS adt_ds (x :: xs) (v :: vs).
+ | EVLamApp
+   :  forall x1 t11 x12 x2 v2 v3
+   ,  EVAL x1 (XLam t11 x12) -> EVAL x2 v2 -> EVAL (substXX 0 v2 x12) v3
+   -> EVAL (XApp x1 x2) v3.
 
 Hint Constructors EVAL.
-Hint Constructors EVALS.
 
 
-(* Invert all hypothesis that are compound eval statements. *)
-Ltac inverts_eval :=
- repeat
-  (match goal with
-   | [ H: EVAL (XApp _ _)  _ |- _ ] => inverts H
-   | [ H: EVAL (XCon _ _)  _ |- _ ] => inverts H
-   | [ H: EVAL (XMatch _ _) _ |- _ ] => inverts H
-   end).
-
-
-(* Theorem EVAL_mutind *)
-(*  :  forall (PE : exp      -> exp      -> Prop) *)
-(*            (PS : list exp -> list exp -> Prop) *)
-
-(*  ,  (forall v2 *)
-(*     ,  wnfX v2 *)
-(*     -> PE v2 v2) *)
-(*  -> (forall x1 t11 x12 x2 v2 v3 *)
-(*     ,  EVAL x1 (XLam t11 x12)    -> PE x1 (XLam t11 x12) *)
-(*     -> EVAL x2 v2                -> PE x2 v2 *)
-(*     -> EVAL (substX 0 v2 x12) v3 -> PE (substX 0 v2 x12) v3 *)
-(*     -> PE (XApp x1 x2) v3) *)
-(*  -> (forall x1 x11 t1 t2 x2 v2 v3, *)
-(*        EVAL x1 (XFix t1 t2 x11) -> PE x1 (XFix t1 t2 x11) *)
-(*        -> EVAL x2 v2 -> PE x2 v2 *)
-(*        -> EVAL (substX 0 (XFix t1 t2 x11) (substX 0 v2 x11)) v3 -> PE (substX 0 (XFix t1 t2 x11) (substX 0 v2 x11)) v3 *)
-(*        -> PE (XApp x1 x2) v3) *)
-(*  -> (forall dc xs vs *)
-(*     ,  EVALS xs vs               -> PS xs vs *)
-(*     -> PE (XCon dc xs) (XCon dc vs)) *)
-(*  -> (forall x1 x2 v3 dc vs alts tsArgs *)
-(*     ,  EVAL x1 (XCon dc vs)      -> PE x1 (XCon dc vs) *)
-(*     -> Forall wnfX vs *)
-(*     -> getAlt dc alts = Some (AAlt dc tsArgs x2) *)
-(*     -> EVAL (substXs 0 vs x2) v3 -> PE (substXs 0 vs x2) v3 *)
-(*     -> PE (XMatch x1 alts) v3) *)
-(*  (* -> (forall t1 t2 x1 v1 x2 pr, *) *)
-(*  (*       EVAL x1 (XChoice t1 t2 pr) -> PE x1 (XChoice t1 t2 pr) *) *)
-(*  (*       -> wnf v1 *) *)
-(*  (*       -> pr x2 *) *)
-(*  (*   ) *) *)
-
-(*  -> (  PS nil nil) *)
-(*  -> (forall x v xs vs *)
-(*     ,  EVAL x v                  -> PE x  v *)
-(*     -> EVALS xs vs               -> PS xs vs *)
-(*     -> PS (x :: xs) (v :: vs)) *)
-(*  -> forall x1 x2 *)
-(*  ,  EVAL x1 x2 -> PE x1 x2. *)
-
-(* Proof. *)
-(*  intros PE PS. *)
-(*  intros Hdone Hlam Hcon Hcase Hnil Hcons. *)
-(*  refine (fix  IHPE x  x'  (HE: EVAL  x  x')  {struct HE} *)
-(*               : PE x x'   := _ *)
-(*          with IHPS xs xs' (HS: EVALS xs xs') {struct HS} *)
-(*               : PS xs xs' := _ *)
-(*          for  IHPE). *)
-
-(*  case HE; intros. *)
-(*  eapply Hdone; eauto. *)
-(*  eapply Hlam;  eauto. *)
-(*  eapply Hcon;  eauto. *)
-(*  eapply Hcase; eauto. *)
-
-(*  case HS; intros. *)
-(*  eapply Hnil. *)
-(*  eapply Hcons; eauto. *)
-(* Qed. *)
-(* Admitted. *)
-
-(* A terminating big-step evaluation always produces a whnf.
+(* A terminating big-step evaluation always produces a wnf.
    The fact that the evaluation terminated is implied by the fact
-   that we have a finite proof of EVAL to pass to this lemma. *)
+   that we have a finite proof of EVAL to pass to this lemma.
+ *)
 Lemma eval_produces_wnfX
- :  forall adt_ds x1 v1
- ,  EVAL adt_ds   x1 v1
+ :  forall x1 v1
+ ,  EVAL   x1 v1
  -> wnfX  v1.
 Proof.
-(*  intros. *)
-(*  induction H using EVAL_mutind with *)
-(*   (PS := fun xs vs *)
-(*       => EVALS xs vs *)
-(*       -> Forall wnfX vs); *)
-(*   intros; eauto. *)
-(* Qed. *)
-Admitted.
+ intros. induction H; eauto.
+Qed.
 Hint Resolve eval_produces_wnfX.
 
 
-Lemma evals_produces_wnfX
- :  forall adt_ds xs vs
- ,  EVALS adt_ds xs vs
- -> Forall wnfX vs.
-Proof.
-  (* intros. induction H; eauto. Qed. *)
-Admitted.
-Hint Resolve evals_produces_wnfX.
-
-
-(* Big to Small steps
-   Convert a big-step evaluation into a list of individual
-   machine steps. *)
+(********************************************************************)
+(* Convert a big-step evaluation into a list of small steps. *)
 Lemma steps_of_eval
-  : forall alg_ds adt_ds x1 t1 x2,
-    TYPE alg_ds adt_ds nil x1 t1
-    -> EVAL adt_ds x1 x2
- -> STEPS adt_ds x1 x2.
+ :  forall x1 t1 x2
+ ,  TYPE nil nil x1 t1
+ -> EVAL  x1 x2
+ -> STEPS x1 x2.
 Proof.
-(*  intros ds x1 t1 v2 HT HE. gen t1. *)
-(*  induction HE using EVAL_mutind with *)
-(*   (PS := fun xs vs => forall ts *)
-(*       ,  Forall2 (TYPE ds nil) xs ts *)
-(*       -> EVALS xs vs *)
-(*       -> Forall2 STEPS xs vs) *)
-(*   ; intros. *)
+ intros x1 t1 v2 HT HE. gen t1.
 
-(*  Case "EvDone". *)
-(*   intros. apply EsNone. *)
+ (* Induction over the form of (EVAL x1 x2) *)
+ induction HE.
+ Case "EVDone".
+  intros. apply ESNone.
 
-(*  (* Function Application ***) *)
-(*  Case "EvLamApp". *)
-(*   intros. inverts HT. *)
+ Case "EVLAMAPP".
+  intros. inverts HT.
+  lets E1: IHHE1 H3. clear IHHE1.
+  lets T1: preservation_steps H3 E1. inverts keep T1.
+  lets T2: subst_type_value H4 H5.
+   simpl in T2.
+  lets E2: IHHE2 T2.
+  eapply ESAppend.
+   apply steps_APP1. eauto.
+  eapply ESAppend.
+   eapply ESStep.
+    eapply ESLAMAPP. auto.
 
-(*   lets E1: IHHE1 H3. *)
-(*   lets E2: IHHE2 H5. *)
-(*   lets T1: preservation_steps H3 E1. inverts keep T1. *)
-(*   lets T2: preservation_steps H5 E2. *)
-(*   lets T3: subst_exp_exp H2 T2. *)
-(*   lets E3: IHHE3 T3. *)
-
-(*   eapply EsAppend. *)
-(*     lets D: steps_context XcApp1. eapply D. eauto. *)
-(*    eapply EsAppend. *)
-(*     lets D: steps_context (XcApp2 (XLam t0 x12)). eauto. *)
-(*     eapply D. eauto. *)
-(*    eapply EsAppend. *)
-(*     eapply EsStep. *)
-(*      eapply EsLamApp. eauto. eauto. *)
-
-(*  (* Constructor evaluation ***) *)
-(*  Case "EvCon". *)
-(*   intros. *)
-(*   inverts HT. *)
-(*   lets D: IHHE H8 H. *)
-(*   eapply steps_in_XCon; eauto. *)
-
-
-(*  (* Case selection ***) *)
-(*  Case "EvCase". *)
-(*   intros. inverts keep HT. *)
-
-(*   lets Ex1: IHHE1 H3. clear IHHE1. *)
-
-(*   eapply EsAppend. *)
-(*    (* evaluate the discriminant *) *)
-(*    lets HSx1: steps_context XcCase. eapply HSx1. *)
-(*     eapply Ex1. *)
-
-(*   (* choose the alternative *) *)
-(*   lets HTCon: preservation_steps H3 Ex1. clear Ex1. *)
-(*   inverts HTCon. *)
-(*   assert (tsArgs0 = tsArgs). *)
-(*    eapply getAlt_ctorArgTypesMatchDataDef; eauto. subst. *)
-
-(*   lets HA: getAlt_in H0. *)
-(*   norm. rip. *)
-(*   apply H4 in HA. *)
-(*   inverts HA. *)
-
-(*    (* substitute ctor values into alternative *) *)
-(*   eapply EsAppend. *)
-(*    eapply EsStep. *)
-(*     eapply EsCaseAlt; burn. *)
-(*      burn using subst_exp_exp_list. *)
-
-(*  Case "EvsNil". *)
-(*   auto. *)
-
-(*  Case "EvsHead". *)
-(*   destruct ts. *)
-(*    inverts H0. *)
-(*    inverts H0. eauto. *)
-(* Qed. *)
-Admitted.
+ Case "EVLamApp".
+  intros. inverts HT.
+  lets E1: IHHE1 H3.
+  lets E2: IHHE2 H5.
+  lets T1: preservation_steps H3 E1. inverts keep T1.
+  lets T2: preservation_steps H5 E2.
+  lets T3: subst_value_value H8 T2.
+  lets E3: IHHE3 T3.
+  eapply ESAppend.
+    eapply steps_app1. eauto.
+   eapply ESAppend.
+    eapply steps_app2. eauto. eauto.
+   eapply ESAppend.
+    eapply ESStep.
+     eapply ESLamApp. eauto.
+   eauto.
+Qed.
 
 
-(* Small to Big steps
-   Convert a list of individual machine steps to a big-step
-   evaluation. The main part of this is the expansion lemma, which
-   we use to build up the overall big-step evaluation one small-step
-   at a time. The other lemmas are used to feed it small-steps. *)
+(********************************************************************)
+(* Convert a list of small steps to a big-step evaluation. The main
+   part of this is the expansion lemma, which we use to build up the
+   overall big-step evaluation one small-step at a time. The other
+  lemmas are used to feed it small-steps.
+ *)
 
 (* Given an existing big-step evalution, we can produce a new one
    that does an extra step before returning the original value.
  *)
 Lemma eval_expansion
-  : forall alg_ds adt_ds te x1 t1 x2 v3,
-    TYPE alg_ds adt_ds te x1 t1
- -> STEP adt_ds x1 x2 -> EVAL adt_ds x2 v3
- -> EVAL adt_ds x1 v3.
+ :  forall ke te x1 t1 x2 v3
+ ,  TYPE ke te x1 t1
+ -> STEP x1 x2 -> EVAL x2 v3
+ -> EVAL x1 v3.
 Proof.
-(*  intros ds te x1 t1 x2 v3 HT HS. gen ds te t1 v3. *)
-(*  induction HS; intros; *)
-(*   try (solve [inverts H; eauto]); *)
-(*   try eauto. *)
+ intros. gen ke te t1 v3.
 
-(*  Case "Context". *)
-(*   destruct H; inverts_type; eauto. *)
+ (* Induction over the form of (STEP x1 x2) *)
+ induction H0; intros.
 
-(*    SCase "XcApp1". *)
-(*     inverts_eval; burn. *)
+ Case "XApp".
+  SCase "value app".
+   eapply EVLamApp.
+   eauto.
+   inverts H.
+   apply EVDone. auto. auto.
 
-(*    SCase "XcApp2". *)
-(*     inverts_eval; burn. *)
+  SCase "x1 steps".
+   inverts H. inverts H1.
+    inverts H.
+    eapply EVLamApp; eauto.
 
-(*    SCase "XcCon". *)
-(*     assert (exists t, TYPE ds te x t). *)
-(*     eapply exps_ctx_Forall2_exists_left; eauto. *)
-(*     dest t. *)
+  SCase "x2 steps".
+   inverts H1. inverts H2.
+   inverts H1.
+   eapply EVLamApp; eauto.
 
-(*     inverts_eval. *)
-(*     inverts H2. *)
-(*     eapply EvCon. clear H9. *)
+ Case "XAPP".
+  SCase "type app".
+   eapply EVLAMAPP.
+   eauto.
+   inverts H.
+   auto.
 
-(*     induction H; intros. *)
-(*       inverts H5. *)
-(*       eapply EvsCons. eauto. *)
-(*        induction xs. *)
-(*         eauto. *)
-(*         inverts H6. eauto. *)
-(*         inverts H5. eauto. *)
+  SCase "x1 steps".
+   inverts H. inverts H1.
+    inverts H.
+    eapply EVLAMAPP; eauto.
+Qed.
 
-(*     eapply EvCon. *)
-(*      clear H3 H4 H9. *)
-(*      gen vs. *)
-(*      induction H; intros. *)
-(*       inverts H8. eauto. *)
-(*       inverts H8. eauto. *)
-
-(*    SCase "XcCase". *)
-(*     inverts H0. inverts H. eauto. *)
-(* Qed. *)
-Admitted.
 
 (* Convert a list of small steps to a big-step evaluation. *)
 Lemma eval_of_stepsl
-  : forall alg_ds adt_ds x1 t1 v2,
-    TYPE alg_ds adt_ds nil x1 t1
-    -> STEPSL adt_ds x1 v2 -> value v2
-    -> EVAL adt_ds   x1 v2.
+ :  forall x1 t1 v2
+ ,  TYPE nil nil x1 t1
+ -> STEPSL x1 v2 -> value v2
+ -> EVAL   x1 v2.
 Proof.
-(*  intros. *)
-(*  induction H0. *)
+ intros.
+ induction H0.
 
-(*  Case "EslNone". *)
-(*   apply EvDone. inverts H1. auto. *)
+ Case "ESLNone".
+   apply EVDone. inverts H1. auto.
 
-(*  Case "EslCons". *)
-(*   eapply eval_expansion; eauto. *)
-(*   burn using preservation. *)
-(* Qed. *)
-Admitted.
+ Case "ESLCons".
+  eapply eval_expansion.
+   eauto. eauto.
+   apply IHSTEPSL.
+   eapply preservation. eauto. auto. auto.
+Qed.
+
 
 (* Convert a multi-step evaluation to a big-step evaluation.
    We use stepsl_of_steps to flatten out the append constructors
    in the multi-step evaluation, leaving a list of individual
-   small-steps. *)
+   small-steps.
+ *)
 Lemma eval_of_steps
-  : forall alg_ds adt_ds x1 t1 v2,
-    TYPE alg_ds adt_ds nil x1 t1
-    -> STEPS adt_ds x1 v2 -> value v2
-    -> EVAL adt_ds  x1 v2.
+ :  forall x1 t1 v2
+ ,  TYPE nil nil x1 t1
+ -> STEPS x1 v2 -> value v2
+ -> EVAL  x1 v2.
 Proof.
-(*  intros. *)
-(*  eapply eval_of_stepsl; eauto. *)
-(*  apply  stepsl_of_steps; auto. *)
-(* Qed. *)
-Admitted.
+ intros.
+ eapply eval_of_stepsl; eauto.
+ apply  stepsl_of_steps; auto.
+Qed.
