FiatFormal/Language/Exp.v
@@ -1,137 +1,53 @@
 
-Require Export FiatFormal.Language.ExpBase.
-Require Export FiatFormal.Language.ExpLift.
-Require Export FiatFormal.Language.ExpSubst.
-Require Export FiatFormal.Language.ExpAlt.
+Require Export FiatFormal.Language.TyEnv.
+Require Export FiatFormal.Language.Ty.
+Require Export FiatFormal.Language.Ki.
 
-(* Weak normal forms cannot be reduced further by
+
+(* Expressions *)
+Inductive exp : Type :=
+ | XVar  : nat -> exp             (* deBruijn indices *)
+ | XLAM  : exp -> exp             (* Type abstraction *)
+ | XAPP  : exp -> ty  -> exp      (* Type application *)
+ | XLam  : ty  -> exp -> exp      (* Value abstraction *)
+ | XApp  : exp -> exp -> exp.     (* Value application *)
+
+Hint Constructors exp.
+
+
+(* Weak normal dorms cannot be reduced further by
    call-by-value evaluation. *)
 Inductive wnfX : exp -> Prop :=
  | Wnf_XVar
    : forall i
    , wnfX (XVar i)
 
- (* | Wnf_XLam *)
- (*   : forall t1 x2 *)
- (*   , wnfX (XLam t1 x2) *)
+ | Wnf_XLAM
+   : forall x1
+   , wnfX (XLAM x1)
 
- | Wnf_XNaryFun
-   : forall tsArgs x,
-     wnfX (XNaryFun tsArgs x)
+ | Wnf_XLam
+   : forall t1 x2
+   , wnfX (XLam t1 x2).
 
- | Wnf_XFix
-   : forall t1 t2 x1
-   , wnfX (XFix t1 t2 x1)
-
- | Wnf_XCon
-   :  forall dc xs
-   ,  Forall wnfX xs
-      -> wnfX (XCon dc xs)
-
- | Wnf_XPair
-   : forall x1 x2,
-     wnfX x1
-     -> wnfX x2
-     -> wnfX (XPair x1 x2).
 Hint Constructors wnfX.
 
 
-(* Well formed expressions are closed under the given environment. *)
-Inductive wfX : tyenv -> exp -> Prop :=
- | WfX_Let
-   : forall te ac n x,
-     wfX te x
-     -> wfX te (XLet ac n x)
-
- | WfX_XVar
-   :  forall te i
-   ,  (exists t, get i te = Some t)
-   -> wfX te (XVar i)
-
- | WfX_XFix
-   : forall te t1 t2 x1
-   , wfX (te :> (TFun t1 t2) :> t1) x1
-     -> wfX te (XFix t1 t2 x1)
-
- | WfX_XNaryFun
-   : forall te tsArgs x,
-     wfX (te >< tsArgs) x
-     -> wfX te (XNaryFun tsArgs x)
-
- | WfX_XNaryApp
-   : forall te x1 xs,
-     wfX te x1 -> Forall (wfX te) xs
-     -> wfX te (XNaryApp x1 xs)
-
- | WfX_XApp
-   :  forall te x1 x2
-   ,  wfX te x1 -> wfX te x2
-   -> wfX te (XApp x1 x2)
-
- | WfX_XCon
-   :  forall te dc xs
-   ,  Forall (wfX te) xs
-   -> wfX te (XCon dc xs)
-
- | WfX_XMatch
-   :  forall te x alts
-   ,  wfX te x
-   -> Forall (wfA te) alts
-   -> wfX te (XMatch x alts)
-
- | WfX_XChoice
-   : forall te t1 xs fp,
-     Forall (wfX te) xs
-     -> wfP te fp
-     -> wfX te (XChoice t1 xs fp)
-
- | WfX_XPair
-   : forall te x1 x2,
-     wfX te x1
-     -> wfX te x2
-     -> wfX te (XPair x1 x2)
-
- | WfX_XFst
-   : forall te x1,
-     wfX te x1
-     -> wfX te (XFst x1)
-
- | WfX_XSnd
-   : forall te x1,
-     wfX te x1
-     -> wfX te (XSnd x1)
-
- (* | WfX_XOpCall *)
- (*   : forall adt_ds x s te ac n xs, *)
- (*     getADTBody ac n adt_ds  = Some x *)
- (*     -> getADTSig ac n adt_ds = Some s *)
- (*     (* Having appropriate size of tyenv all the matters here *) *)
- (*     -> wfX nil x *)
- (*     -> length xs = s.(arity) + length(s.(dom)) *)
- (*     -> Forall (wfX te) xs *)
- (*     -> wfX te (XOpCall ac n xs) *)
-
-with    wfA : tyenv -> alt -> Prop :=
- | WfA_AAlt
-   : forall te dc ds ts x tsArgs tResult,
-     getDataDef dc ds = Some (DefData dc tsArgs tResult)
-     -> wfX (te >< tsArgs) x
-     -> length ts = length tsArgs (* TODO: consider whether *)
-                                (* necessary. needed in one of my lemmas  *)
-     -> wfA te (AAlt dc ts x)
-
-with wfP : tyenv -> fpred -> Prop :=
-     | WfP_FPred
-       : forall pc x te,
-         wfP te (FPred pc x).
-
-Hint Constructors wfX.
-Hint Constructors wfA.
+(* A well formed expression is closed under the given environments *)
+Fixpoint wfX (ke: kienv) (te: tyenv) (xx: exp) : Prop :=
+ match xx with
+ | XVar i     => exists t, get i te = Some t
+ | XLAM x     => wfX (ke :> KStar) (liftTE 0 te) x
+ | XAPP x t   => wfX ke te x  /\ wfT ke t
+ | XLam t x   => wfT ke t     /\ wfX ke (te :> t) x
+ | XApp x1 x2 => wfX ke te x1 /\ wfX ke te x2
+ end.
+Hint Unfold wfX.
 
 
-(* Closed expressions are well formed under an empty environment. *)
+(* Closed expressions are well formed under empty environments *)
 Definition closedX (xx: exp) : Prop
- := wfX nil xx.
+ := wfX nil nil xx.
 Hint Unfold closedX.
 
 
@@ -143,96 +59,96 @@ Inductive value : exp -> Prop :=
    -> value xx.
 Hint Constructors value.
 
-Lemma value_wnfX
- : forall xx, value xx -> wnfX xx.
-Proof.
-  intros. inverts H. auto. Qed.
-Hint Resolve value_wnfX.
 
-Lemma value_closedX
- : forall xx, value xx -> closedX xx.
-Proof.
-  intros. inverts H. auto. Qed.
-Hint Resolve value_closedX.
+(********************************************************************)
+(* Lift type indices in expressions. *)
+Fixpoint liftTX (d: nat) (xx: exp) : exp :=
+  match xx with
+  |  XVar _     => xx
 
-Lemma value_wnfXs_XCon
- : forall xs dc
- , value (XCon dc xs) -> Forall wnfX xs.
-Proof.
- intros. inverts H. inverts H0. auto.
-Qed.
-Hint Resolve value_wnfXs_XCon.
+  (* Increase type depth when moving across type abstractions. *)
+  |  XLAM x
+  => XLAM (liftTX (S d) x)
 
-Lemma value_closedXs_XCon
- : forall xs dc
- , value (XCon dc xs) -> Forall closedX xs.
-Proof.
- intros. inverts H. inverts H1. auto.
-Qed.
-Hint Resolve value_closedXs_XCon.
+  |  XAPP x t
+  => XAPP (liftTX d x)  (liftTT d t)
 
-(* Invert all hypothesis that are compound well-formedness statements. *)
-Ltac inverts_wfX :=
- repeat
-  (match goal with
-   | [H: wfX _  (XLet _)         |- _ ] => inverts H
-   | [ H: wfX _ (XVar  _)        |- _ ] => inverts H
-   | [ H: wfX _ (XFix _ _ _)     |- _ ] => inverts H
-   | [ H: wfX _ (XApp  _ _)      |- _ ] => inverts H
-   | [ H: wfX _ (XCon  _ _)      |- _ ] => inverts H
-   | [ H: wfX _ (XMatch _ _)     |- _ ] => inverts H
-   | [ H: wfX _ (XChoice _ _ _)  |- _ ] => inverts H
-   | [ H: wfA _ (AAlt _ _ _)     |- _ ] => inverts H
-   | [ H: wfX _ (XPair _ _)      |- _ ] => inverts H
-   | [ H: wfX _ (XFst _)         |- _ ] => inverts H
-   | [ H: wfX _ (XSnd _)         |- _ ] => inverts H
-   (* | [ H: wfX _ (XOpCall _ _ _)    |- _ ] => inverts H *)
-   | [ H: wfP _ (FPred _ _)      |- _ ] => inverts H
-   end).
+  |  XLam t x
+  => XLam (liftTT d t)  (liftTX d x)
 
-(* Lemma liftX_closed_pmk *)
-(*   : forall x n te, *)
-(*     wfX te x -> (liftX n (length te) x) = x. *)
-(* Proof. *)
-(*   intros x n. *)
-(*   gen n. *)
-(*   induction x using exp_mutind with *)
-(*      (PA := fun a => forall n te, wfA te a -> (liftA n (length te) a) = a) *)
-(*      (PF := fun f => f = f); intros; rip; burn; subst. *)
-(*   inverts_wfX. dest t. *)
-(*   simpl. *)
-(*   fbreak_le_gt_dec; auto. *)
-(*   pose proof (get_above_false _ _ _ _ l H); nope. *)
-(*   inverts_wfX. *)
-(*   spec IHx H2. simpl in *; subst. *)
-(*   erewrite IHx; burn. *)
-(*   inverts_wfX; simpl. *)
-(*   spec IHx1 H3; spec IHx2 H4; espread; burn. *)
-(*   inverts_wfX; repeat nforall. *)
-(*   simpl. *)
+  |  XApp x1 x2
+  => XApp (liftTX d x1) (liftTX d x2)
+ end.
 
-(*   assert (forall x, In x xs -> liftX n (length te) x = x). *)
-(*   intros. apply H. assumption. spec H3 H0. assumption. *)
-(*   pose proof (map_ext_in _ _ xs H0). *)
-(*   rewrite H1. *)
-(*   rewrite map_id; burn. *)
 
-(*   simpl. *)
-(*   inverts_wfX. *)
-(*   repeat nforall. *)
+(* Lift value indices in expressions. *)
+Fixpoint liftXX (d: nat) (xx: exp) : exp :=
+  match xx with
+  |  XVar ix
+  => if le_gt_dec d ix
+      then XVar (S ix)
+      else xx
 
-(*   assert (forall a, In a aa -> liftA n (length te) a = a). *)
-(*   intros. apply H. assumption. spec H5 H0. assumption. *)
-(*   pose proof (map_ext_in _ _ aa H0). *)
-(*   rewrite H1. *)
-(*   rewrite map_id. *)
-(*   spec IHx H4. espread; burn. *)
+  |  XLAM x
+  => XLAM (liftXX d x)
 
-(*   simpl. *)
-(*   inverts_wfX. *)
-(*   assert (liftX n (length (te >< ts)) x = x). *)
-(*   eapply IHx. *)
-(*   pose proof (getAlt_ctorArgTypesMatchDataDef _ _ _ _). *)
-(*   eapply IHx. *)
+  |  XAPP x t
+  => XAPP (liftXX d x) t
 
-(*   Admitted. *)
+  (* Increase value depth when moving across value abstractions. *)
+  |  XLam t x
+  => XLam t (liftXX (S d) x)
+
+  |  XApp x1 x2
+  => XApp (liftXX d x1) (liftXX d x2)
+ end.
+
+
+(********************************************************************)
+(* Substitution of types in expressions. *)
+Fixpoint substTX (d: nat) (u: ty) (xx: exp) : exp :=
+  match xx with
+  | XVar _     => xx
+
+  (* Lift free type variables in the type to be substituted
+     when we move across type abstractions. *)
+  |  XLAM x
+  => XLAM (substTX (S d) (liftTT 0 u) x)
+
+  |  XAPP x t
+  => XAPP (substTX d u x)  (substTT d u t)
+
+  |  XLam t x
+  => XLam (substTT d u t)  (substTX d u x)
+
+  |  XApp x1 x2
+  => XApp (substTX d u x1) (substTX d u x2)
+ end.
+
+
+(* Substitution of expressions in expressions. *)
+Fixpoint substXX (d: nat) (u: exp) (xx: exp) : exp :=
+  match xx with
+  | XVar ix
+  => match nat_compare ix d with
+     | Eq => u
+     | Gt => XVar (ix - 1)
+     | _  => XVar  ix
+     end
+
+  (* Lift free type variables in the expression to be substituted
+     when we move across type abstractions. *)
+  |  XLAM x
+  => XLAM (substXX d (liftTX 0 u) x)
+
+  |  XAPP x t
+  => XAPP (substXX d u x) t
+
+  (* Lift free value variables in the expression to be substituted
+     when we move across value abstractions. *)
+  |  XLam t x
+  => XLam t (substXX (S d) (liftXX 0 u) x)
+
+  |  XApp x1 x2
+  => XApp (substXX d u x1) (substXX d u x2)
+  end.
