FiatFormal/Language/Step.v
@@ -1,244 +1,157 @@
 
-Require Export FiatFormal.Language.StepContext.
-Require Export FiatFormal.Language.StepAlt.
-Require Export FiatFormal.Language.TyJudge.
-Require Export FiatFormal.Language.SubstExpExp.
+Require Import FiatFormal.Language.SubstTypeExp.
+Require Import FiatFormal.Language.SubstExpExp.
 Require Export FiatFormal.Language.Exp.
 
 
-(** * Single Small Step Evaluation *)
-(** The single step rules model the individual transitions that the
-     machine can make at runtime. *)
+(* Small step evaluation *)
+Inductive STEP : exp -> exp -> Prop :=
+  (* value applications *)
+  | ESLamApp
+    :  forall t11 x12 v2
+    ,  value v2
+    -> STEP (XApp (XLam t11 x12) v2) (substXX 0 v2 x12)
 
-Inductive STEP : adt_defs -> exp -> exp -> Prop :=
+  | ESApp1
+    :  forall x1 x1' x2
+    ,  STEP x1 x1'
+    -> STEP (XApp x1 x2) (XApp x1' x2)
 
- (* Step some sub-expression in an evaluation context *)
- | EsContext
-   :  forall adt_ds C x x',
-     exp_ctx C
-   -> STEP adt_ds x x'
-   -> STEP adt_ds (C x) (C x')
+  | ESApp2
+    :  forall v1 x2 x2'
+    ,  value v1
+    -> STEP x2 x2'
+    -> STEP (XApp v1 x2) (XApp v1 x2')
 
- | EsLet
-   : forall adt_ds ac n  b x,
-     getADTBody ac n adt_ds = Some b
-     -> STEP adt_ds (XLet ac n x) (methodSubstX ac n b x) (* previously needed to subst all methods here *)
+  (* type applications *)
+  | ESLAMAPP
+    :  forall x12 t2
+    ,  STEP (XAPP (XLAM x12) t2) (substTX 0 t2 x12)
 
- | EsFixApp
-   : forall adt_ds t1 t2 x1 v1,
-     wnfX v1
-     -> STEP adt_ds (XApp (XFix t1 t2 x1) v1)
-            (substX 0 (XFix t1 t2 x1) (substX 0 v1 x1))
-
- | EsMatchAlt
-   :  forall adt_ds dc vs tsArgs alts x,
-     Forall wnfX vs
-   -> getAlt dc alts = Some (AAlt dc tsArgs x)
-   -> STEP adt_ds (XMatch (XCon dc vs) alts)
-          (substXs 0 vs x)
-
- | EsPairFst
-   : forall adt_ds v1 v2,
-     wnfX v1
-     -> wnfX v2
-     -> STEP adt_ds (XFst (XPair v1 v2)) v1
-
- | EsPairSnd
-   : forall adt_ds v1 v2,
-     wnfX v1
-     -> wnfX v2
-     -> STEP adt_ds (XSnd (XPair v1 v2)) v2
-
- (* | EsADTCall *)
- (*   : forall adt_ds ac n vs x, *)
- (*     Forall wnfX vs *)
- (*   -> getADTBody ac n adt_ds = Some x *)
- (*   -> STEP adt_ds (XCall ac n vs) (substXs 0 vs x) *)
-
- | EsChoice
-   : forall adt_ds t1 xs fp,
-     STEP adt_ds (XChoice t1 xs fp) (XChoice t1 xs fp)
-     (* fp = FiatPred t11 pr -> *)
-     (* exists xDenoted v1, wnfX v1 /\ pr t1 xDenoted *)
-     (*                    -> STEP (XChoice t1 xs fp) v1 *)
-.
+  | ESAPP1
+    :  forall x1 x1' t2
+    ,  STEP x1 x1'
+    -> STEP (XAPP x1 t2) (XAPP x1' t2).
 
 Hint Constructors STEP.
 
 
-(* Multi-step evaluation
+(********************************************************************)
+(* Multi-step evaluation.
    A sequence of small step transitions.
    As opposed to STEPSL, this version has an append constructor
    ESAppend that makes it easy to join two evaluations together.
-   We use this when converting big-step evaluations to small-step. *)
-Inductive STEPS : adt_defs -> exp -> exp -> Prop :=
+   We use this when converting big-step evaluations to small-step.
+ *)
+Inductive STEPS : exp -> exp -> Prop :=
 
  (* After no steps, we get the same exp.
     We need this constructor to match the EVDone constructor
     in the big-step evaluation, so we can convert between big-step
     and multi-step evaluations. *)
- | EsNone
-   :  forall adt_ds x1,
-     STEPS adt_ds x1 x1
+ | ESNone
+   :  forall x1
+   ,  STEPS x1 x1
 
  (* Take a single step. *)
- | EsStep
-   :  forall adt_ds x1 x2,
-     STEP adt_ds x1 x2
-   -> STEPS adt_ds x1 x2
+ | ESStep
+   :  forall x1 x2
+   ,  STEP  x1 x2
+   -> STEPS x1 x2
 
  (* Combine two evaluations into a third. *)
- | EsAppend
-   :  forall adt_ds x1 x2 x3,
-     STEPS adt_ds x1 x2 -> STEPS adt_ds x2 x3
-   -> STEPS adt_ds x1 x3.
+ | ESAppend
+   :  forall x1 x2 x3
+   ,  STEPS x1 x2 -> STEPS x2 x3
+   -> STEPS x1 x3.
 
 Hint Constructors STEPS.
 
 
-(* Stepping a wnf doesn't change it. *)
-Lemma step_wnfX
-  : forall adt_ds x v,
-    wnfX x -> STEP adt_ds x v -> v = x.
+(* Context lemmas
+   These help when proving something about a reduction in a given
+   context. They're all trivial.
+   TODO: Define contexts directly like in the Simple proof.
+ *)
+Lemma steps_app1
+ :  forall x1 x1' x2
+ ,  STEPS x1 x1'
+ -> STEPS (XApp x1 x2) (XApp x1' x2).
 Proof.
-(*  intros x v HW HS. *)
-(*  induction HS; nope. *)
-(*   destruct H; burn. *)
-
-(*  Case "XCon dc (C x)". *)
-(*   inverts HW. *)
-(*   assert (wnfX x). *)
-(*   eapply exps_ctx_Forall; eauto. *)
-(*   rrwrite (x' = x). auto. *)
-(* Qed. *)
-Admitted.
+ intros. induction H; eauto.
+Qed.
+Hint Resolve steps_app1.
 
 
-Lemma step_context_XCon_exists
-  : forall adt_ds C x dc,
-    exps_ctx wnfX C
-    -> (exists x', STEP adt_ds x x')
-    -> (exists x', STEP adt_ds (XCon dc (C x)) (XCon dc (C x'))).
+Lemma steps_app2
+ :  forall v1 x2 x2'
+ ,  value v1
+ -> STEPS x2 x2'
+ -> STEPS (XApp v1 x2) (XApp v1 x2').
 Proof.
- intros adt_ds C x dc HC HS.
- shift x'.
- eapply (EsContext adt_ds (fun xx => XCon dc (C xx))); auto.
+ intros. induction H0; eauto.
+Qed.
+Hint Resolve steps_app2.
+
+
+Lemma steps_APP1
+ :  forall x1 x1' t2
+ ,  STEPS x1 x1'
+ -> STEPS (XAPP x1 t2) (XAPP x1' t2).
+Proof.
+ intros. induction H; eauto.
 Qed.
 
-Lemma step_context_XCall_exists_pmk
-  : forall adt_ds C x ac n,
-    exps_ctx wnfX C
-    -> (exists x', STEP adt_ds x x')
-    -> (exists x', STEP adt_ds (XOpCall ac n (C x)) (XOpCall ac n (C x'))).
-Proof.
- intros adt_ds C x ac n HC HS.
- shift x'.
- eapply (EsContext adt_ds (fun xx => XOpCall ac n (C xx))); auto.
-Qed.
-
-
-(* Multi-step evaluating a wnf doesn't change it. *)
-Lemma steps_wnfX
-  : forall adt_ds x v,
-    wnfX x -> STEPS adt_ds x v -> v = x.
-Proof.
-(*  intros x v HW HS. *)
-(*  induction HS; burn. *)
-(*   Case "EsStep". *)
-(*    apply step_wnfX; auto. *)
-
-(*   Case "EsAppend". *)
-(*    have (x2 = x1). subst. auto. *)
-(* Qed. *)
-Admitted.
-
-(* Multi-step evaluation in a context. *)
-Lemma steps_context
-  : forall adt_ds C x1 x1',
-    exp_ctx C
-    -> STEPS adt_ds x1 x1'
-    -> STEPS adt_ds (C x1) (C x1').
-Proof.
-(*  intros C x1 x1' HC HS. *)
-(*  induction HS; eauto. *)
-(* Qed. *)
-Admitted.
-
-(* Multi-step evaluation of a data constructor argument. *)
-Lemma steps_context_XCon
-  : forall adt_ds C x v dc,
-    exps_ctx wnfX C
-    -> STEPS adt_ds x v
-    -> STEPS adt_ds (XCon dc (C x)) (XCon dc (C v)).
-Proof.
-(*  intros C x v dc HC HS. *)
-(*  induction HS; auto. *)
-
-(*  Case "XCon". *)
-(*   lets D: EsContext XcCon; eauto.  *)
-(*   eauto. *)
-(* Qed. *)
-Admitted.
-
-Lemma steps_in_XCon
-  : forall adt_ds xs vs dc,
-    Forall2 (STEPS adt_ds) xs vs
-    -> Forall wnfX vs
-    -> STEPS adt_ds (XCon dc xs) (XCon dc vs).
-Proof.
-(*  intros xs vs dc HS HW. *)
-(*  lets HC: make_chain HS HW. *)
-(*   eapply steps_wnfX. *)
-
-(*  clear HS. clear HW. *)
-(*  induction HC; auto. *)
-(*   eapply (EsAppend (XCon dc (C x)) (XCon dc (C v))); auto. *)
-(*   eapply steps_context_XCon; auto. *)
-(* Qed. *)
-Admitted.
 
 (********************************************************************)
 (* Left linearised multi-step evaluation
    As opposed to STEPS, this version provides a single step at a time
    and does not have an append constructor. This is convenient
-   when converting small-step evaluations to big-step, via the
-   eval_expansion lemma. *)
-Inductive STEPSL : adt_defs -> exp -> exp -> Prop :=
- | EslNone
-   : forall adt_ds x1,
-     STEPSL adt_ds x1 x1
+   when converting a small-step evaluations to big-step, via the
+   eval_expansion lemma.
+ *)
+Inductive STEPSL : exp -> exp -> Prop :=
 
- | EslCons
-   : forall adt_ds x1 x2 x3,
-     STEP adt_ds x1 x2 -> STEPSL adt_ds x2 x3
-   -> STEPSL adt_ds x1 x3.
+ | ESLNone
+   : forall x1
+   , STEPSL x1 x1
+
+ | ESLCons
+   :  forall x1 x2 x3
+   ,  STEP   x1 x2 -> STEPSL x2 x3
+   -> STEPSL x1 x3.
 
 Hint Constructors STEPSL.
 
 
 (* Transitivity of left linearised multi-step evaluation.
    We use this when "flattening" a big step evaluation to the
-   small step one. *)
+   small step one.
+ *)
 Lemma stepsl_trans
-  : forall adt_ds x1 x2 x3,
-    STEPSL adt_ds x1 x2 -> STEPSL adt_ds x2 x3
- -> STEPSL adt_ds x1 x3.
+ :  forall x1 x2 x3
+ ,  STEPSL x1 x2 -> STEPSL x2 x3
+ -> STEPSL x1 x3.
 Proof.
-(*  intros x1 x2 x3 H1 H2. *)
-(*  induction H1; eauto. *)
-(* Qed. *)
-Admitted.
+ intros.
+ induction H.
+  eauto.
+  eapply ESLCons. eauto. eauto.
+Qed.
+
 
 (* Linearise a regular multi-step evaluation.
    This flattens out all the append constructors, leaving us with
-   a list of individual transitions. *)
+   a list of individual transitions.
+ *)
 Lemma stepsl_of_steps
-  : forall adt_ds x1 x2,
-    STEPS adt_ds x1 x2
-    -> STEPSL adt_ds x1 x2.
+ :  forall x1 x2
+ ,  STEPS  x1 x2
+ -> STEPSL x1 x2.
 Proof.
-(*  intros x1 x2 HS. *)
-(*  induction HS;  *)
-(*   eauto using stepsl_trans. *)
-(* Qed. *)
-Admitted.
+ intros.
+ induction H.
+  auto.
+  eauto.
+  eapply stepsl_trans; eauto.
+Qed.
