FiatFormal/Language/TyJudge.v
@@ -1,421 +1,197 @@
-(* TODO/NOTES
 
-Switching order of forall binding changes typechecking result.
-
-This type checks:
-
- | TYProg
-   : forall alg_ds adt_ds d ac pf te r x t,
-     TYPE alg_ds adt_ds te x t
-     -> getADTRep ac adt_ds d pf = r
-     -> TYPE_ADT alg_ds adt_ds ac
-     -> TYPE alg_ds adt_ds te x t
-     -> TYPE alg_ds adt_ds te (XLet ac x) (typeSubst ac r t)
-
-This does not:
-
- | TYProg
-   : forall alg_ds adt_ds d pf ac te r x t,
-     TYPE alg_ds adt_ds te x t
-     -> getADTRep ac adt_ds d pf = r
-     -> TYPE_ADT alg_ds adt_ds ac
-     -> TYPE alg_ds adt_ds te x t
-     -> TYPE alg_ds adt_ds te (XLet ac x) (typeSubst ac r t)
-
-*)
-
+Require Import FiatFormal.Language.SubstTypeType.
+Require Export FiatFormal.Language.KiJudge.
+Require Export FiatFormal.Language.TyEnv.
 Require Export FiatFormal.Language.Exp.
 
-(* Type Judgement assigns a type to an expression. *)
-Inductive TYPE : alg_defs -> adt_defs -> tyenv -> exp -> ty -> Prop :=
- (* Variables *)
+
+(* Type judgement assigns a type to an expression. *)
+Inductive TYPE : kienv -> tyenv -> exp -> ty -> Prop :=
  | TYVar
-   :  forall alg_ds adt_ds te i t,
-     get i te = Some t
-   -> TYPE alg_ds adt_ds te (XVar i) t
+   :  forall i ke te t
+   ,  get i te = Some t
+   -> KIND ke t  KStar
+   -> TYPE ke te (XVar i) t
 
- | TYFix
-   : forall alg_ds adt_ds te t1 t2 x1,
-     TYPE alg_ds adt_ds (te :> (TFun t1 t2) :> t1) x1 t2
-     -> TYPE alg_ds adt_ds te (XFix t1 t2 x1) (TFun t1 t2)
+ | TYLam
+   :  forall ke te x12 t11 t12
+   ,  KIND ke t11 KStar
+   -> TYPE ke (te :> t11)  x12            t12
+   -> TYPE ke  te         (XLam t11 x12) (TFun t11 t12)
 
- (* Applications *)
  | TYApp
-   :  forall alg_ds adt_ds te x1 x2 t1 t2,
-     TYPE alg_ds adt_ds te x1           (TFun t1 t2)
-   -> TYPE alg_ds adt_ds te x2           t1
-   -> TYPE alg_ds adt_ds te (XApp x1 x2) t2
+   :  forall ke te x1 x2 t11 t12
+   ,  TYPE ke te x1 (TFun t11 t12)
+   -> TYPE ke te x2 t11
+   -> TYPE ke te (XApp x1 x2) t12
 
- | TYNaryFun
-   : forall alg_ds adt_ds te x tsArgs tResult,
-     TYPE alg_ds adt_ds (te >< tsArgs) x         tResult
-     -> TYPE alg_ds adt_ds te (XNaryFun tsArgs x) (TNaryFun tsArgs tResult)
+ | TYLAM
+   :  forall ke te x1 t1
+   ,  TYPE (ke :> KStar) (liftTE 0 te) x1        t1
+   -> TYPE ke            te           (XLAM x1) (TForall t1)
 
- | TYNaryApp
-   :  forall alg_ds adt_ds te x xs tsArgs t2,
-     TYPE alg_ds adt_ds te x           (TNaryFun tsArgs t2)
-   -> Forall2 (TYPE alg_ds adt_ds te) xs tsArgs
-   -> TYPE alg_ds adt_ds te (XNaryApp x xs) t2
-
- (* Data Constructors *)
- | TYCon
-   :  forall alg_ds adt_ds te xs dc dcs tsArgs tc,
-     getDataDef dc alg_ds = Some (DefData     dc tsArgs (TCon tc))
-   -> getTypeDef tc alg_ds = Some (DefDataType tc dcs)
-   -> In dc dcs
-   -> Forall2 (TYPE alg_ds adt_ds te) xs tsArgs
-   -> TYPE alg_ds adt_ds te (XCon dc xs) (TCon tc)
-
- (* Match Expressions *)
- | TYMatch
-   :  forall alg_ds adt_ds te xObj tcPat tResult alts dcs,
-
-      (* check types of expression and alternatives *)
-     TYPE alg_ds adt_ds te xObj (TCon tcPat)
-   -> Forall (fun alt => TYPEA alg_ds adt_ds te alt (TCon tcPat) tResult) alts
-
-      (* there must be at least one alternative *)
-   -> length alts > 0
-
-      (* all data cons must have a corresponding alternative *)
-   -> getTypeDef tcPat alg_ds = Some (DefDataType tcPat dcs)
-   -> Forall (fun dc => In dc (map dcOfAlt alts)) dcs
-
-   -> TYPE alg_ds adt_ds te (XMatch xObj alts) tResult
-
- | TYChoice
-   : forall alg_ds adt_ds t1 t2 xs te P ts,
-     TYPEP alg_ds adt_ds te P t2
-     -> Forall2 (TYPE alg_ds adt_ds te) xs ts
-     -> TYPE alg_ds adt_ds te (XChoice t1 xs P) t1
-
- | TYPair
-   : forall alg_ds adt_ds te t1 t2 x1 x2,
-     TYPE alg_ds adt_ds te x1 t1
-     -> TYPE alg_ds adt_ds te x2 t2
-     -> TYPE alg_ds adt_ds te (XPair x1 x2) (TProd t1 t2)
-
- | TYFst
-   : forall alg_ds adt_ds te t1 t2 x,
-     TYPE alg_ds adt_ds te x (TProd t1 t2)
-     -> TYPE alg_ds adt_ds te (XFst x) t1
-
- | TYSnd
-   : forall alg_ds adt_ds te t1 t2 x,
-     TYPE alg_ds adt_ds te x (TProd t1 t2)
-     -> TYPE alg_ds adt_ds te (XSnd x) t2
-
- | TYOpCall
-   : forall alg_ds adt_ds ac n te r s xs tsArgs tResult,
-     getADTSig ac n adt_ds = Some s
-     -> getADTRep ac adt_ds = Some r
-     -> sigToNaryFunTy r s = TNaryFun tsArgs tResult
-     -> Forall2 (TYPE alg_ds adt_ds te) xs tsArgs
-     -> TYPE alg_ds adt_ds te (XOpCall ac n xs) tResult
-
- | TYProg
-   : forall alg_ds adt_ds ac n te r x t,
-     TYPE alg_ds adt_ds te x t
-     -> getADTRep ac adt_ds = Some r
-     -> TYPE_ADT alg_ds adt_ds ac
-     -> TYPE alg_ds adt_ds te x t
-     -> TYPE alg_ds adt_ds te (XLet ac n x) (typeSubst ac r t)
-
-with TYPE_ADT : alg_defs -> adt_defs -> adtcon -> Prop :=
-     | TYAdt : forall alg_ds adt_ds ac ss bs r,
-         getADTBodies ac adt_ds = Some bs
-         -> getADTSigs ac adt_ds = Some ss
-         -> getADTRep ac adt_ds = Some r
-         -> Forall2 (TYPE alg_ds adt_ds nil) bs (map (sigToNaryFunTy r) ss)
-         -> TYPE_ADT alg_ds adt_ds ac
-
-with TYPEP : alg_defs -> adt_defs -> tyenv -> fpred -> ty -> Prop :=
-     (* placeholder for predicate typing -- this is old *)
-     | TYPred : forall alg_ds adt_ds te pc x,
-         TYPEP alg_ds adt_ds te (FPred pc x) (TPred pc)
-
-with TYPEA : alg_defs -> adt_defs -> tyenv -> alt -> ty -> ty -> Prop :=
-     (* Match Alternatives *)
-     | TYAlt
-       :  forall alg_ds adt_ds te x1 t1 dc tsArgs tResult,
-         getDataDef dc alg_ds = Some (DefData dc tsArgs tResult)
-         -> TYPE  alg_ds adt_ds (te >< tsArgs) x1 t1
-         -> TYPEA alg_ds adt_ds te (AAlt dc tsArgs x1) tResult t1.
+ | TYAPP
+   :  forall ke te x1 t1 t2
+   ,  TYPE ke te x1 (TForall t1)
+   -> KIND ke t2 KStar
+   -> TYPE ke te (XAPP x1 t2) (substTT 0 t2 t1).
 
 Hint Constructors TYPE.
-Hint Constructors TYPEA.
-Hint Constructors TYPEP.
 
 
-(* Invert all hypothesis that are compound typing statements. *)
-Ltac inverts_type :=
- repeat
-  (match goal with
-   | [ H: TYPE _ _ _ (XVar  _)    _    |- _ ] => inverts H
-   (* | [ H: TYPE _ _ _ (XLam  _ _)  _    |- _ ] => inverts H *)
-   | [ H: TYPE _ _ _ (XFix _ _ _)  _    |- _ ] => inverts H
-   | [ H: TYPE _ _ _ (XNaryFun _ _)  _    |- _ ] => inverts H
-   | [ H: TYPE _ _ _ (XNaryApp _ _)  _    |- _ ] => inverts H
-   | [ H: TYPE _ _ _ (XApp  _ _)  _    |- _ ] => inverts H
-   | [ H: TYPE _ _ _ (XCon  _ _)  _    |- _ ] => inverts H
-   | [ H: TYPE _ _ _ (XMatch _ _)  _    |- _ ] => inverts H
-   | [ H: TYPE _ _ _ (XChoice _ _ _) _  |- _ ] => inverts H
-   | [ H: TYPEA _ _ _ (AAlt _ _ _) _ _  |- _ ] => inverts H
-   | [ H: TYPE _ _ _ (XPair _ _) _      |- _ ] => inverts H
-   | [ H: TYPE _ _ _ (XFst _) _         |- _ ] => inverts H
-   | [ H: TYPE _ _ _ (XSnd _) _         |- _ ] => inverts H
-   | [ H: TYPE _ _ _ (XOpCall _ _ _) _ |- _ ] => inverts H
-   | [ H: TYPEP _ _ _ (FPred _ _) _ |- _ ] => inverts H
-   | [ H: TYPE _ _ _ (XLet _ _ _) _ |- _ ] => inverts H
-   | [ H: TYPE_ADT _ _ _ _ |- _ ] => inverts H
-   end).
-
-
-(********************************************************************)
-(* Forms of values.
-   If we know the type of a value,
-   then we know the form of that value. *)
-(* Lemma value_lam *)
-(*  :  forall x alg_ds adt_ds te t1 t2 *)
-(*  ,  value x *)
-(*  -> TYPE alg_ds adt_ds te x (TFun t1 t2) *)
-(*  -> (exists t x', x = XLam t x') *)
-(* Proof. *)
-(*  intros. destruct x; burn. *)
-(* Qed. *)
-(* Hint Resolve value_lam. *)
-
-Lemma value_fix
-  : forall x alg_ds adt_ds te t1 t2,
-    value x
-    -> TYPE alg_ds adt_ds te x (TFun t1 t2)
-    -> exists t1 t2 x', x = XFix t1 t2 x'.
+(* The type produced by a type judgement is well kinded. *)
+Theorem type_kind
+ :  forall ke te x t
+ ,  TYPE ke te x t
+ -> KIND ke t KStar.
 Proof.
-  intros. destruct x; burn.
-(* Qed. *)
-Admitted.
-Hint Resolve value_fix.
+ intros. gen ke te t.
+ induction x; intros; inverts H; eauto.
 
-(********************************************************************)
-(* A well typed expression is well formed *)
+ Case "XAPP".
+  apply IHx in H4. inverts H4.
+  eapply subst_type_type; eauto.
+
+ Case "XLam".
+  eapply IHx1 in H4. inverts H4. auto.
+Qed.
+
+
+(* A well typed expression is well formed. *)
 Theorem type_wfX
-  :  forall alg_ds adt_ds te x t,
-    TYPE alg_ds adt_ds te x t
-    -> wfX te x.
+ :  forall ke te x t
+ ,  TYPE ke te x t
+ -> wfX  ke te x.
 Proof.
+ intros. gen ke te t.
+ induction x; intros; simpl.
 
- (* intros. gen alg_ds adt_ds te t. *)
- (* induction x using exp_mutind with *)
- (*     (PA := fun a => forall alg_ds adt_ds te t1 t2, *)
- (*                TYPEA alg_ds adt_ds te a t1 t2 *)
- (*                -> wfA te a) *)
- (*     (PF := fun f => forall alg_ds adt_ds te t1, *)
- (*                TYPEP alg_ds adt_ds te f t1 *)
- (*                -> wfP te f) *)
- (*  ; intros; inverts_type; eauto. *)
+ Case "XVar".
+  inverts H. eauto.
 
- (* Case "XCon". *)
- (*  apply WfX_XCon. repeat nforall. intros. *)
- (*  have HT: (exists t, TYPE alg_ds adt_ds te x t). *)
- (*  spec H H0 alg_ds adt_ds te. *)
- (*  destruct HT as [t]. *)
- (*  burn. *)
+ Case "XLAM".
+  inverts H.
+  apply IHx in H3. eauto.
 
- (* Case "XMatch". *)
- (*  eapply WfX_XMatch; repeat nforall; burn. *)
+ Case "XAPP".
+  inverts H.
+  lets D: IHx H4. split.
+   auto. eapply kind_wfT. eauto.
 
- (*  Case "XChoice". *)
- (*  apply WfX_XChoice. *)
- (*  repeat nforall; intros. *)
- (*  spec H H0 alg_ds adt_ds te. *)
- (*  pose proof (Forall2_exists_left (TYPE alg_ds adt_ds te)). *)
- (*  spec H1 H0 H9. *)
- (*  destruct H1 as [y]; burn. *)
- (*  eapply IHx; burn. *)
- (*  apply WfP_FPred. *)
+ Case "XLam".
+  inverts H.
+  apply IHx in H6.
+  apply kind_wfT in H4. auto.
 
- (*  Case "XCall". *)
- (*  repeat nforall. *)
-
-
-  (* apply (WfX_XCall adt_ds ). *)
-
-(* Qed. *)
-Admitted.
+ Case "XApp".
+  inverts H.
+  apply IHx1 in H4.
+  apply IHx2 in H6.
+   auto.
+Qed.
 Hint Resolve type_wfX.
 
 
-(* Weakening Type Env in Type Judgement.
-   We can insert a new type into the type environment, provided we
-   lift existing references to types higher in the stack across
-   the new one. *)
+(********************************************************************)
+(* Weakening the kind environment of a type judgement.
+   We can insert a new kind into the kind environment of a type
+   judgement, provided we lift existing references to kinds higher
+   than this in the stack over the new one.
+
+   References to existing elements of the kind environment may
+   appear in the type environment, expression, as well as the
+   resulting type -- so we must lift all of them.
+ *)
+Lemma type_kienv_insert
+ :  forall ix ke te x1 t1 k2
+ ,  TYPE ke                 te             x1             t1
+ -> TYPE (insert ix k2 ke) (liftTE ix te) (liftTX ix x1) (liftTT ix t1).
+Proof.
+ intros. gen ix ke te t1 k2.
+ induction x1; intros; inverts H; simpl; eauto.
+
+ Case "XVar".
+  apply TYVar.
+  apply get_map. auto.
+  apply liftTT_insert. auto.
+
+ Case "XLAM".
+  eapply TYLAM.
+  rewrite insert_rewind.
+   rewrite (liftTE_liftTE 0 ix).
+   apply IHx1. auto.
+
+ Case "XAPP".
+  rewrite (liftTT_substTT' 0 ix). simpl.
+  eapply TYAPP.
+  eapply (IHx1 ix) in H4. simpl in H4. eauto.
+  apply liftTT_insert. auto.
+
+ Case "XLam".
+  apply TYLam.
+   apply liftTT_insert. auto.
+   assert ( liftTE ix te :> liftTT ix t
+          = liftTE ix (te :> t)). auto. rewrite H. clear H.
+   apply IHx1. auto.
+
+ Case "XApp".
+  eapply TYApp.
+   eapply IHx1_1 in H4. simpl in H4. eauto.
+   eapply IHx1_2 in H6. eauto.
+Qed.
+
+
+Lemma type_kienv_weaken
+ :  forall ke te x1 t1 k2
+ ,  TYPE ke         te            x1            t1
+ -> TYPE (ke :> k2) (liftTE 0 te) (liftTX 0 x1) (liftTT 0 t1).
+Proof.
+ intros.
+ assert (ke :> k2 = insert 0 k2 ke).
+  destruct ke; auto. rewrite H0.
+  apply type_kienv_insert. auto.
+Qed.
+
+
+(********************************************************************)
+(* Weakening the type environment of a type judgement.
+   We can insert a new type into the type environment of a type
+   judgement, provided we lift existing references to types higher
+   than this in the stack over the new one.
+ *)
 Lemma type_tyenv_insert
- :  forall alg_ds adt_ds te ix x t1 t2
- ,  TYPE alg_ds adt_ds te x t1
- -> TYPE alg_ds adt_ds (insert ix t2 te) (liftX 1 ix x) t1.
+ :  forall ke te ix x1 t1 t2
+ ,  TYPE ke  te                x1            t1
+ -> TYPE ke (insert ix t2 te) (liftXX ix x1) t1.
 Proof.
-(*  intros. gen ix ds te t1. *)
-(*  induction x using exp_mutind with  *)
-(*   (PA := fun a => forall ix ds te t3 t4 *)
-(*       ,  TYPEA ds te a t3 t4  *)
-(*       -> TYPEA ds (insert ix t2 te) (liftA 1 ix a) t3 t4) *)
-(*   ; intros; inverts_type; burn; simpl. *)
+ intros. gen ix ke te t1 t2.
+ induction x1; intros; simpl; inverts H; eauto.
 
-(*  Case "XVar". *)
-(*   lift_cases; burn. *)
+ Case "XVar".
+  lift_cases; intros; auto.
 
-(*  Case "XLam". *)
-(*   apply TYLam. *)
-(*   rewrite insert_rewind. auto. *)
+ Case "XLAM".
+  apply TYLAM. simpl.
+  assert ( liftTE 0 (insert ix t2 te)
+         = insert ix (liftTT 0 t2) (liftTE 0 te)).
+   unfold liftTE. rewrite map_insert. auto.
+  rewrite H.
+  apply IHx1. auto.
 
-(*  Case "XCon". *)
-(*   eapply TYCon; burn. *)
-(*    apply (Forall2_map_left (TYPE ds (insert ix t2 te))). *)
-(*    apply (Forall2_impl_in  (TYPE ds te)); eauto. *)
-(*    nforall. eauto. *)
+ Case "XLam".
+  eapply TYLam.
+   auto.
+   rewrite insert_rewind. apply IHx1. auto.
+Qed.
 
-(*  Case "XCase". *)
-(*   eapply TYCase; eauto. *)
-(*    apply Forall_map. *)
-(*    apply (Forall_impl_in (fun a => TYPEA ds te a (TCon tcPat) t1)); eauto. *)
-(*    repeat nforall. burn. *)
 
-(*   rewrite map_length; auto. *)
-
-(*   norm. *)
-(*    intros. rename x0 into d.  *)
-(*    rewrite map_map. unfold Basics.compose. *)
-(*    eapply map_exists_in. *)
-(*    have (In d (map dcOfAlt aa)).  *)
-(*    assert (exists a, dcOfAlt a = d /\ In a aa). *)
-(*     eapply map_in_exists. auto. *)
-(*    shift a. rip. *)
-(*    eapply dcOfAlt_liftA. *)
-
-(*  Case "XAlt". *)
-(*   eapply TYAlt; eauto. *)
-(*   rewrite insert_app. auto. *)
-(* Qed.  *)
-Admitted.
-
-(* We can push a new type onto the environment stack provided
-   we lift references to existing types across the new one. *)
-Lemma type_tyenv_weaken1
- :  forall alg_ds adt_ds te x t1 t2
- ,  TYPE alg_ds adt_ds te x t1
- -> TYPE alg_ds adt_ds (te :> t2) (liftX 1 0 x) t1.
+Lemma type_tyenv_weaken
+ :  forall ke te x1 t1 t2
+ ,  TYPE ke  te         x1           t1
+ -> TYPE ke (te :> t2) (liftXX 0 x1) t1.
 Proof.
-(*  intros. *)
-(*  rrwrite (te :> t2 = insert 0 t2 te). *)
-(*  burn using type_tyenv_insert. *)
-(* Qed. *)
-Admitted.
-
-(* We can push several new types onto the environment stack provided
-   we lift referenes to existing types across the new one. *)
-Lemma type_tyenv_weaken_append
- :  forall alg_ds adt_ds te te' x t1
- ,  TYPE alg_ds adt_ds te x t1
- -> TYPE alg_ds adt_ds (te >< te') (liftX (length te') 0 x) t1.
-Proof.
-(*  intros. *)
-(*  induction te'; simpl. *)
-(*  rewrite liftX_zero; auto. *)
-(*  rewrite <- nat_plus_one. *)
-(*  rrwrite (length te' + 1 = 1 + length te'). *)
-(*  rewrite <- liftX_plus. *)
-(*  eapply type_tyenv_weaken1. auto.  *)
-(* Qed. *)
-Admitted.
-
-(* ---------------------------------------------------------- *)
-
-Definition buildNaryApp x xs :=
-  XNaryApp x xs.
-
-Lemma type_method_type_nary :
-  forall alg_ds adt_ds ac n te xs b tResult,
-    TYPE alg_ds adt_ds te (XOpCall ac n xs) tResult
-    -> getADTBody ac n adt_ds = Some b
-    -> TYPE_ADT alg_ds adt_ds ac
-    -> TYPE alg_ds adt_ds te (buildNaryApp b xs) tResult.
-Proof.
-  intros. unfold buildNaryApp.
-  eapply TYNaryApp.
-  inversion H; subst.
-  inversion H1; subst.
-  rewrite H9 in H4. norm_inverts_option.
-Admitted.
-
-Lemma adt_x_in_xs :
-  forall ac n adt_ds b bs,
-    getADTBody ac n adt_ds = Some b
-    -> getADTBodies ac adt_ds = Some bs
-    -> In b bs.
-Proof.
-  intros. unfold getADTBody, getADTBodies in *.
-  induction bs.
-Admitted.
-
-(* Lemma wellTypedCallHasBody_pmk : forall ac n alg_ds adt_ds te xs t, *)
-(*     TYPE alg_ds adt_ds te (XOpCall ac n xs) t -> *)
-(*     exists b, getADTBody ac n adt_ds = Some b. *)
-(* Proof. *)
-  (* intros. *)
-  (* inverts_type; burn. *)
-(* Admitted. *)
-(* Qed. *)
-
-
-Fixpoint methodSubstX ac n s x : exp :=
-  match x with
-  | XOpCall ac' n' xs => if andb (adtcon_beq ac ac') (beq_nat n n')
-                        then (buildNaryApp s xs)
-                        else XOpCall ac' n' (map (methodSubstX ac n s) xs)
-  | XLet ac' n' x' => XLet ac' n' (methodSubstX ac n s x')
-  | XNaryFun tsArgs x' => XNaryFun tsArgs (methodSubstX ac n s x')
-  | XNaryApp x' xs => XNaryApp (methodSubstX ac n s x') (map (methodSubstX ac n s) xs)
-  | XFix t1 t2 x' => XFix t1 t2 (methodSubstX ac n s x')
-  | XApp x1 x2 => XApp (methodSubstX ac n s x1) (methodSubstX ac n s x2)
-  | XVar n => XVar n
-  | XCon dc xs => XCon dc (map (methodSubstX ac n s) xs)
-  | XMatch x' aa => XMatch (methodSubstX ac n s x') (map (methodSubstA ac n s) aa)
-  | XChoice t1 xs fp => XChoice t1 xs fp (* TODO *)
-  | XPair x1 x2 => XPair (methodSubstX ac n s x1) (methodSubstX ac n s x2)
-  | XFst x' => XFst (methodSubstX ac n s x')
-  | XSnd x' => XSnd (methodSubstX ac n s x')
-  end
-with methodSubstA ac n s a : alt :=
-       match a with
-       | AAlt dc ts x
-         => AAlt dc ts (methodSubstX ac n s x)
-       end.
-
-(* Fixpoint methodSubstX ac n adt_ds b d pf (pre : getADTBody ac n adt_ds d pf = Some b) (x : exp) : exp := *)
-(*   match x with *)
-(*   | XOpCall ac' n' xs => if andb (adtcon_beq ac ac') (beq_nat n n') *)
-(*                         then (buildNaryApp b xs) *)
-(*                         else XOpCall ac' n' (map (methodSubstX ac n adt_ds b pre) xs) *)
-(*   | XLet ac' x' => XLet ac (methodSubstX ac n adt_ds b pre x') *)
-(*   | XNaryFun tsArgs x' => XNaryFun tsArgs (methodSubstX ac n adt_ds b pre x') *)
-(*   | XNaryApp x' xs => XNaryApp (methodSubstX ac n adt_ds b pre x') (map (methodSubstX ac n adt_ds b pre) xs) *)
-(*   | XFix t1 t2 x' => XFix t1 t2 (methodSubstX ac n adt_ds b pre x') *)
-(*   | XApp x1 x2 => XApp (methodSubstX ac n adt_ds b pre x1) (methodSubstX ac n adt_ds b pre x2) *)
-(*   | XVar n => XVar n *)
-(*   | XCon dc xs => XCon dc (map (methodSubstX ac n adt_ds b pre) xs) *)
-(*   | XMatch x' aa => XMatch (methodSubstX ac n adt_ds b pre x') (map (methodSubstA ac n adt_ds b pre) aa) *)
-(*   | XChoice t1 xs fp => XChoice t1 xs fp (* TODO *) *)
-(*   | XPair x1 x2 => XPair (methodSubstX ac n adt_ds b pre x1) (methodSubstX ac n adt_ds b pre x2) *)
-(*   | XFst x' => XFst (methodSubstX ac n adt_ds b pre x') *)
-(*   | XSnd x' => XSnd (methodSubstX ac n adt_ds b pre x') *)
-(*   end *)
-
-(* with methodSubstA ac n adt_ds b d pf (pre : getADTBody ac n adt_ds d pf = Some b) (a : alt) : alt := *)
-(*        match a with *)
-(*        | AAlt dc ts x *)
-(*          => AAlt dc ts (methodSubstX ac n adt_ds b pre x) *)
-(*        end. *)
-
-(* Fixpoint methodsToFunctions (ac : adtcon) (adt_ds : adt_defs) (d : adt_def) (pre : getADTDef ac adt_ds = Some d) (x : exp) : exp := *)
-(*   match pre with *)
-(*   | _ => *)
+ intros.
+ assert (te :> t2 = insert 0 t2 te).
+  destruct te; auto. rewrite H0.
+  apply type_tyenv_insert. auto.
+Qed.
