FiatFormal/Language/Base.v
@@ -1,39 +1,9 @@
-Require Export FiatFormal.PMKList.
 
 Require Export FiatFormal.Data.List.
 Require Export FiatFormal.Data.Nat.
-Require Export FiatFormal.Norm.List.
 Require Export FiatFormal.Norm.
-Require Export FiatFormal.Tactics.Rip2.
-Require Export FiatFormal.Tactics.Rewrite2.
-Require Export FiatFormal.Tactics.Case.
-Require Export FiatFormal.Tactics.Nope.
-Require Export FiatFormal.Tactics.Break.
-Require Export FiatFormal.Tactics.Rewrite.
-Require Export FiatFormal.Tactics.Have.
-Require Export FiatFormal.Tactics.Exists.
-Require Export FiatFormal.Tactics.Short.
 Require Export FiatFormal.Tactics.LibTactics.
-Require Export Coq.Arith.EqNat.
+Require Export FiatFormal.Tactics.Have.
+Require Export FiatFormal.Tactics.Rip2.
+Require Export Coq.Program.Basics.
 Require Export Coq.Arith.Compare_dec.
-Require Export Coq.Logic.FunctionalExtensionality.
-
-
-Ltac norm
- := simpl in *;
-    repeat (rip; try norm_nat; try norm_lists).
-
-Ltac tburn0 T
- := norm; eauto using T; nope.
-
-Ltac tburn T
- := try (solve [ tburn0 T
-               | red; tburn0 T]).
-
-Tactic Notation "burn"
- := tburn false.
-
-Tactic Notation "burn" "using" tactic(T)
- := tburn T.
-
-Ltac have_auto ::= burn.
