FiatFormal/Language/Preservation.v
@@ -1,108 +1,88 @@
 
 Require Import FiatFormal.Language.Step.
-Require Import FiatFormal.Language.TyJudge.
 Require Import FiatFormal.Language.SubstExpExp.
+Require Import FiatFormal.Language.SubstTypeExp.
+Require Import FiatFormal.Language.SubstTypeType.
+Require Import FiatFormal.Language.TyJudge.
 
 
-(* When a well typed expression transitions to the next state
-   then its type is preserved. *)
+(* When an expression takes a step the results has the same type. *)
 Theorem preservation
-  : forall alg_ds adt_ds x x' t,
-    TYPE alg_ds adt_ds nil x  t
- -> STEP adt_ds x x'
- -> TYPE alg_ds adt_ds nil x' t.
+ :  forall ke te x x' t
+ ,  TYPE ke te x t
+ -> STEP x x'
+ -> TYPE ke te x' t.
 Proof.
- intros alg_ds adt_ds x x' t HT HS. gen t.
- induction HS; intros; inverts_type; eauto.
+ intros ke te x x' t HT HS.
+ gen ke te x' t.
+ induction x; intros.
 
- (* Evaluation in an arbitrary context. *)
- Case "EsContext".
-  destruct H; inverts_type; eauto.
+ Case "XVar".
+  inverts HS.
 
-  SCase "XCon".
-   eapply TYCon; eauto.
-   eapply exps_ctx_Forall2_swap; eauto.
-  SCase "EsOpCall".
-  admit.
+ Case "XLAM".
+  inverts HS.
 
- (* Case "EsLamApp". *)
- (*  eapply subst_exp_exp; eauto. *)
+ Case "XAPP".
+  inverts HT.
+  inverts keep HS.
 
-  Case "XLet".
-  inversion H9; subst.
+  SCase "ESAPPLAM".
+   inverts H3.
+   eapply subst_type_value in H4; eauto.
+   rewrite substTE_liftTE in H4. auto.
 
-  Case "XFix".
-  repeat (eapply subst_exp_exp); eauto.
-  pose proof (type_tyenv_weaken1).
-  pose proof (H0 alg_ds adt_ds nil v1 t0 (TFun t0 t) H7).
-  pose proof (type_wfX _ _ _ _ _ H7).
-  pose proof (liftX_closed_pmk v1 1 nil H2); simpl in *. rewrite <- H3.
-  assumption.
+  SCase "ESAPP1".
+   apply TYAPP; eauto.
 
- Case "EsMatchAlt".
-  eapply subst_exp_exp_list; eauto.
-  eapply getAlt_bodyIsWellTyped_fromCase; eauto.
-  assert (tsArgs = tsArgs0).
-   lets D: getAlt_ctorArgTypesMatchDataDef H4 H7 H0. auto.
-   subst. auto.
+ Case "XLam".
+  inverts HS.
 
- Case "XCallBody".
- repeat nforall.
- eapply subst_exp_exp_list; eauto.
- assert (XB: x = b); burn; subst.
+ Case "XApp".
+  inverts HT.
+  inverts keep HS.
 
- admit.
+  SCase "ESAppLam".
+   inverts H3.
+   lets D: subst_value_value H9 H5. auto.
 
-(* Qed. *)
-Admitted.
-(* ORIG *)
-(*  intros ds x x' t HT HS. gen t. *)
-(*  induction HS; intros; inverts_type; eauto. *)
+  SCase "EsApp1".
+   eapply TYApp; eauto.
 
-(*  (* Evaluation in an arbitrary context. *) *)
-(*  Case "EsContext". *)
-(*   destruct H; inverts_type; eauto.  *)
-
-(*   SCase "XCon". *)
-(*    eapply TYCon; eauto. *)
-(*    eapply exps_ctx_Forall2_swap; eauto. *)
-
-(*  Case "EsLamApp". *)
-(*   eapply subst_exp_exp; eauto. *)
-
-(*  Case "EsCaseAlt". *)
-(*   eapply subst_exp_exp_list; eauto. *)
-(*   eapply getAlt_bodyIsWellTyped_fromCase; eauto. *)
-(*   assert (tsArgs = tsArgs0). *)
-(*    lets D: getAlt_ctorArgTypesMatchDataDef H4 H7 H0. auto. *)
-(*    subst. auto. *)
-(* Qed. *)
+  SCase "EsApp2".
+   eapply TYApp; eauto.
+Qed.
 
 
 (* When we multi-step evaluate some expression,
-   then the result has the same type as the original. *)
+   then the result has the same type as the original.
+ *)
 Lemma preservation_steps
-  : forall alg_ds adt_ds x1 t1 x2,
-    TYPE alg_ds adt_ds nil x1 t1
-    -> STEPS adt_ds       x1 x2
-    -> TYPE alg_ds adt_ds nil x2 t1.
+ :  forall x1 t1 x2
+ ,  TYPE nil nil x1 t1
+ -> STEPS x1 x2
+ -> TYPE nil nil x2 t1.
 Proof.
-(*  intros ds x1 t1 x2 HT HS. *)
-(*  induction HS; eauto using preservation. *)
-(* Qed. *)
-Admitted.
+ intros.
+ induction H0; eauto.
+  eapply preservation; eauto.
+Qed.
+
 
 (* When we multi-step evaluate some expression,
    then the result has the same type as the original.
    Using the left-linearised form for the evaluation.
  *)
 Lemma preservation_stepsl
-  : forall alg_ds adt_ds x1 t1 x2,
-    TYPE alg_ds adt_ds nil x1 t1
-    -> STEPSL adt_ds x1 x2
-    -> TYPE alg_ds adt_ds nil x2 t1.
+ :  forall x1 t1 x2
+ ,  TYPE nil nil x1 t1
+ -> STEPSL x1 x2
+ -> TYPE nil nil x2 t1.
 Proof.
-(*  intros ds x1 t1 x2 HT HSL. *)
-(*  induction HSL; eauto using preservation. *)
-(* Qed. *)
-Admitted.
+ intros.
+ induction H0.
+  auto.
+  apply IHSTEPSL.
+  eapply preservation.
+   eauto. auto.
+Qed.
