FiatFormal/Language/SubstExpExp.v
@@ -1,206 +1,63 @@
 
+Require Import FiatFormal.Language.SubstTypeType.
+Require Import FiatFormal.Language.SubstTypeExp.
 Require Import FiatFormal.Language.TyJudge.
-Require Import FiatFormal.Language.ExpSubst.
-Require Export FiatFormal.Language.Exp.
 
 
-(* Substitution of values in values.
-   Inductively, we must reason about performing substitutions at any
-   depth, hence we must prove a property about (subst' d x2 x1) instead
-   of the weaker (subst x2 x1) which assumes the substitution is taking
-   place at top level. *)
-Theorem subst_exp_exp_ix
-  :  forall ix alg_ds adt_ds te x1 x2 t1 t2,
-    get  ix te = Some t2
-    -> TYPE alg_ds adt_ds te           x1 t1
-    -> TYPE alg_ds adt_ds (delete ix te) x2 t2
-    -> TYPE alg_ds adt_ds (delete ix te) (substX ix x2 x1) t1.
+(* Substitution of Values in Values preserves Typing ****************)
+Theorem subst_value_value_ix
+ :  forall ix ke te x1 t1 x2 t2
+ ,  get  ix te = Some t2
+ -> TYPE ke te           x1 t1
+ -> TYPE ke (delete ix te) x2 t2
+ -> TYPE ke (delete ix te) (substXX ix x2 x1) t1.
 Proof.
-(*  intros. gen ix ds te x2 t1 t2. *)
-(*  induction x1 using exp_mutind with *)
-(*   (PA := fun a1 => forall ix ds te x2 t11 t12 t2 *)
-(*       ,  get ix te = Some t2 *)
-(*       -> TYPEA ds te           a1 t11 t12 *)
-(*       -> TYPE  ds (delete ix te) x2 t2 *)
-(*       -> TYPEA ds (delete ix te) (substA ix x2 a1) t11 t12) *)
-(*   ; intros; simpl; inverts_type; eauto. *)
+ intros. gen ix ke te t1 x2 t2.
+ induction x1; intros; inverts H0; simpl; eauto.
 
-(*  Case "XVar". *)
-(*   fbreak_nat_compare; burn. *)
+ Case "XVar".
+  fbreak_nat_compare.
+  SCase "n = ix".
+   rewrite H in H3. inverts H3. auto.
 
-(*   SCase "n > ix". *)
-(*    apply TYVar. *)
-(*    destruct n; burn. *)
-(*    norm. down. apply get_delete_below. omega. *)
+  SCase "n < ix".
+   apply TYVar.
+   rewrite <- H3. apply get_delete_above. auto. auto.
 
-(*  Case "XLam". *)
-(*   apply TYLam. *)
-(*   rewrite delete_rewind. *)
-(*   eauto using type_tyenv_weaken1. *)
+  SCase "n > ix".
+   apply TYVar. auto.
+   rewrite <- H3.
+   destruct n.
+    burn.
+    simpl. nnat. apply get_delete_below. omega.
+    auto.
 
-(*   (* Case "XFix". *) *)
-(*   (* apply TYFix. *) *)
-(*   (* rewrite delete_rewind. *) *)
-(*   (* rewrite delete_rewind. *) *)
-(*   (* eauto using type_tyenv_weaken1. *) *)
+ Case "XLAM".
+  eapply (IHx1 ix) in H5.
+  apply TYLAM.
+   unfold liftTE. rewrite map_delete. eauto.
+   eapply get_map. eauto.
+   unfold liftTE. rewrite <- map_delete.
+    assert (map (liftTT 0) (delete ix te) = liftTE 0 (delete ix te)).
+     unfold liftTE. auto. rewrite H0. clear H0.
+    apply type_kienv_weaken. auto.
 
-(*  Case "XCon". *)
-(*   eapply TYCon; burn. *)
-(*    norm. *)
-(*    apply (Forall2_map_left (TYPE ds (delete ix te))). *)
-(*    apply (Forall2_impl_in  (TYPE ds te)); eauto. *)
-
-(*  (* Case expressions *) *)
-(*  Case "XCase". *)
-(*   eapply TYCase; eauto. *)
-(*    clear IHx1. *)
-
-(*    (* Alts have correct type *) *)
-(*    eapply Forall_map. burn. *)
-
-(*    (* There is at least one alt *) *)
-(*    rewrite map_length; burn. *)
-
-(*    (* Required datacon is in alts list *) *)
-(*    norm. *)
-(*    rename x into d. *)
-(*    rewrite map_map. unfold Basics.compose. *)
-(*    apply in_map_iff. *)
-(*    have (exists a, dcOfAlt a = d /\ In a aa). *)
-(*    shift a. rip. *)
-(*    rewrite dcOfAlt_substA; auto. *)
-
-(*  Case "AAlt". *)
-(*   eapply TYAlt; auto. *)
-(*   rewrite delete_app. *)
-(*   eapply IHx1; eauto. *)
-(*   rewrite <- delete_app. *)
-(*   eauto using type_tyenv_weaken_append. *)
-(* Qed. *)
-Admitted.
-(* ORIG *)
-(*  intros. gen ix ds te x2 t1 t2. *)
-(*  induction x1 using exp_mutind with *)
-(*   (PA := fun a1 => forall ix ds te x2 t11 t12 t2 *)
-(*       ,  get ix te = Some t2 *)
-(*       -> TYPEA ds te           a1 t11 t12 *)
-(*       -> TYPE  ds (delete ix te) x2 t2 *)
-(*       -> TYPEA ds (delete ix te) (substA ix x2 a1) t11 t12) *)
-(*   ; intros; simpl; inverts_type; eauto. *)
-
-(*  Case "XVar". *)
-(*   fbreak_nat_compare; burn. *)
-
-(*   SCase "n > ix". *)
-(*    apply TYVar. *)
-(*    destruct n; burn. *)
-(*    norm. down. apply get_delete_below. omega. *)
-
-(*  Case "XLam". *)
-(*   apply TYLam. *)
-(*   rewrite delete_rewind. *)
-(*   eauto using type_tyenv_weaken1. *)
-
-(*   (* Case "XFix". *) *)
-(*   (* apply TYFix. *) *)
-(*   (* rewrite delete_rewind. *) *)
-(*   (* rewrite delete_rewind. *) *)
-(*   (* eauto using type_tyenv_weaken1. *) *)
-
-(*  Case "XCon". *)
-(*   eapply TYCon; burn. *)
-(*    norm. *)
-(*    apply (Forall2_map_left (TYPE ds (delete ix te))). *)
-(*    apply (Forall2_impl_in  (TYPE ds te)); eauto. *)
-
-(*  (* Case expressions *) *)
-(*  Case "XCase". *)
-(*   eapply TYCase; eauto. *)
-(*    clear IHx1. *)
-
-(*    (* Alts have correct type *) *)
-(*    eapply Forall_map. burn. *)
-
-(*    (* There is at least one alt *) *)
-(*    rewrite map_length; burn. *)
-
-(*    (* Required datacon is in alts list *) *)
-(*    norm. *)
-(*    rename x into d. *)
-(*    rewrite map_map. unfold Basics.compose. *)
-(*    apply in_map_iff. *)
-(*    have (exists a, dcOfAlt a = d /\ In a aa). *)
-(*    shift a. rip. *)
-(*    rewrite dcOfAlt_substA; auto. *)
-
-(*  Case "AAlt". *)
-(*   eapply TYAlt; auto. *)
-(*   rewrite delete_app. *)
-(*   eapply IHx1; eauto. *)
-(*   rewrite <- delete_app. *)
-(*   eauto using type_tyenv_weaken_append. *)
-(* Qed. *)
+ Case "XLam".
+  apply TYLam.
+   auto.
+   rewrite delete_rewind.
+   eapply IHx1; eauto.
+   simpl. apply type_tyenv_weaken. auto.
+Qed.
 
 
-Theorem subst_exp_exp
-  :  forall alg_ds adt_ds te x1 x2 t1 t2,
-    TYPE alg_ds adt_ds (te :> t2) x1 t1
-    -> TYPE alg_ds adt_ds te x2 t2
-    -> TYPE alg_ds adt_ds te (substX 0 x2 x1) t1.
+Theorem subst_value_value
+ :  forall ke te x1 t1 x2 t2
+ ,  TYPE ke (te :> t2) x1 t1
+ -> TYPE ke te x2 t2
+ -> TYPE ke te (substXX 0 x2 x1) t1.
 Proof.
-(*  intros ds te x1 x2 t1 t2 Ht1 Ht2. *)
-(*  lets H: subst_exp_exp_ix 0 (te :> t2). *)
-(*   simpl in H. eauto. *)
-(* Qed. *)
-Admitted.
-
-(* Substitution of several expressions at once. *)
-Theorem subst_exp_exp_list
-  :  forall alg_ds adt_ds te x1 xs t1 ts,
-    Forall2 (TYPE alg_ds adt_ds te) xs ts
-    -> TYPE alg_ds adt_ds (te >< ts) x1 t1
-    -> TYPE alg_ds adt_ds te (substXs 0 xs x1) t1.
-Proof.
-(*  intros ds te x1 xs t1 ts HF HT. *)
-(*  gen ts x1. *)
-(*  induction xs; intros; inverts_type; simpl. *)
-
-(*  Case "base case". *)
-(*   destruct ts; burn. *)
-
-(*  Case "step case". *)
-(*   destruct ts; burn. *)
-(*   simpl in *. *)
-(*   inverts HF. *)
-(*   eapply IHxs. eauto. *)
-(*   eapply subst_exp_exp; eauto. *)
-(*   rrwrite (length xs = length ts). *)
-(*   burn using type_tyenv_weaken_append. *)
-(* Qed. *)
-Admitted.
-
-(* Substitution of several expressions at once, ADT Method version. *)
-(* Theorem subst_exp_exp_list_ADT_pmk *)
-(*   :  forall alg_ds adt_ds te , *)
-(*     Forall2 (TYPE alg_ds adt_ds te) xs (buildMethodTyEnv (TAdt s.(ac)) s) *)
-(*     -> TYPE_ADT alg_ds adt_ds ac *)
-(*     -> TYPE alg_ds adt_ds te (substXs 0 xs x1) s.(cod). *)
-(* Proof. *)
-(*  intros alg_ds adt_ds r s te x1 xs HF HTB. *)
-(*  gen x1 r. *)
-(*  induction xs; intros; inverts_type; simpl. *)
-
-(*  Case "base case". *)
-(*  admit. *)
-(*  (* destruct ts; burn. *) *)
-
-(*  Case "step case". *)
-(*   destruct ts; burn. *)
-(*   simpl in *. *)
-(*   inverts HF. *)
-(*   eapply IHxs. eauto. *)
-(*   eapply subst_exp_exp; eauto. *)
-(*   rrwrite (length xs = length ts). *)
-(*   burn using type_tyenv_weaken_append. *)
-(* (* Qed. *) *)
-(* Admitted. *)
+ intros.
+ assert (te = delete 0 (te :> t2)). auto.
+ rewrite H1. eapply subst_value_value_ix; eauto. eauto.
+Qed.
